Phi_System/IDE_CP_Reasoning1.thy
@@ -241,18 +241,29 @@ text \<open>The process \<^prop>\<open>Remove_Values Input Output\<close> remove
 
 subsection \<open>Collects all Values in an Assertion / from the State Sequent\<close>
 
-consts collect_value :: \<open>unit action\<close>
+consts collect_clean_value :: \<open>unit action\<close>
 
-lemma apply_collect_value:
-  \<open> S \<^bold>i\<^bold>m\<^bold>p\<^bold>l\<^bold>i\<^bold>e\<^bold>s S' \<^bold>a\<^bold>n\<^bold>d V \<^bold><\<^bold>a\<^bold>c\<^bold>t\<^bold>i\<^bold>o\<^bold>n\<^bold>> collect_value
-\<Longrightarrow> PROP Pure.prop (S \<^bold>i\<^bold>m\<^bold>p\<^bold>l\<^bold>i\<^bold>e\<^bold>s S' \<^bold>a\<^bold>n\<^bold>d V)\<close>
-  unfolding 
+lemma apply_collect_clean_value:
+  \<open> S \<^bold>i\<^bold>m\<^bold>p\<^bold>l\<^bold>i\<^bold>e\<^bold>s S' \<^bold>a\<^bold>n\<^bold>d V \<^bold><\<^bold>a\<^bold>c\<^bold>t\<^bold>i\<^bold>o\<^bold>n\<^bold>> collect_clean_value
+\<Longrightarrow> S \<^bold>i\<^bold>m\<^bold>p\<^bold>l\<^bold>i\<^bold>e\<^bold>s S' \<^bold>a\<^bold>n\<^bold>d V\<close>
+  unfolding Action_Tag_def .
 
+lemma [\<phi>reason 1200 for \<open>?S \<heavy_comma> ?x \<Ztypecolon> \<^bold>v\<^bold>a\<^bold>l[?v] ?T \<^bold>i\<^bold>m\<^bold>p\<^bold>l\<^bold>i\<^bold>e\<^bold>s ?S' \<^bold>a\<^bold>n\<^bold>d ?V \<^bold><\<^bold>a\<^bold>c\<^bold>t\<^bold>i\<^bold>o\<^bold>n\<^bold>> collect_clean_value\<close>]:
+  \<open> S \<^bold>i\<^bold>m\<^bold>p\<^bold>l\<^bold>i\<^bold>e\<^bold>s S' \<^bold>a\<^bold>n\<^bold>d V \<^bold><\<^bold>a\<^bold>c\<^bold>t\<^bold>i\<^bold>o\<^bold>n\<^bold>> collect_clean_value
+\<Longrightarrow> S \<heavy_comma> x \<Ztypecolon> \<^bold>v\<^bold>a\<^bold>l[v] T \<^bold>i\<^bold>m\<^bold>p\<^bold>l\<^bold>i\<^bold>e\<^bold>s S' \<^bold>a\<^bold>n\<^bold>d sem_value.dest v \<in> (x \<Ztypecolon> T) \<and> V \<^bold><\<^bold>a\<^bold>c\<^bold>t\<^bold>i\<^bold>o\<^bold>n\<^bold>> collect_clean_value\<close>
+  unfolding Action_Tag_def Imply_def by (clarsimp simp add: \<phi>expns)
 
-lemma Val_inhabited_collect:
-  \<open> Inhabited (x \<Ztypecolon> \<^bold>v\<^bold>a\<^bold>l[v] T) \<Longrightarrow> (sem_value.dest v \<in> (x \<Ztypecolon> T) \<Longrightarrow> C) \<Longrightarrow> C \<close>
-  unfolding Inhabited_def by (clarsimp simp add: \<phi>expns)
+lemma [\<phi>reason 1100 for \<open>?S\<heavy_comma> ?X \<^bold>i\<^bold>m\<^bold>p\<^bold>l\<^bold>i\<^bold>e\<^bold>s ?S' \<^bold>a\<^bold>n\<^bold>d ?V \<^bold><\<^bold>a\<^bold>c\<^bold>t\<^bold>i\<^bold>o\<^bold>n\<^bold>> collect_clean_value\<close>]:
+  \<open> S \<^bold>i\<^bold>m\<^bold>p\<^bold>l\<^bold>i\<^bold>e\<^bold>s S' \<^bold>a\<^bold>n\<^bold>d V \<^bold><\<^bold>a\<^bold>c\<^bold>t\<^bold>i\<^bold>o\<^bold>n\<^bold>> collect_clean_value
+\<Longrightarrow> S\<heavy_comma> X \<^bold>i\<^bold>m\<^bold>p\<^bold>l\<^bold>i\<^bold>e\<^bold>s S'\<heavy_comma> X \<^bold>a\<^bold>n\<^bold>d V \<^bold><\<^bold>a\<^bold>c\<^bold>t\<^bold>i\<^bold>o\<^bold>n\<^bold>> collect_clean_value\<close>
+  unfolding Action_Tag_def using implies_right_prod .
 
+lemma [\<phi>reason 1050 for \<open>?x \<Ztypecolon> \<^bold>v\<^bold>a\<^bold>l[?v] ?T \<^bold>i\<^bold>m\<^bold>p\<^bold>l\<^bold>i\<^bold>e\<^bold>s ?S' \<^bold>a\<^bold>n\<^bold>d ?V \<^bold><\<^bold>a\<^bold>c\<^bold>t\<^bold>i\<^bold>o\<^bold>n\<^bold>> collect_clean_value\<close>]:
+  \<open> x \<Ztypecolon> \<^bold>v\<^bold>a\<^bold>l[v] T \<^bold>i\<^bold>m\<^bold>p\<^bold>l\<^bold>i\<^bold>e\<^bold>s Void \<^bold>a\<^bold>n\<^bold>d sem_value.dest v \<in> (x \<Ztypecolon> T) \<and> True \<^bold><\<^bold>a\<^bold>c\<^bold>t\<^bold>i\<^bold>o\<^bold>n\<^bold>> collect_clean_value \<close>
+  unfolding Action_Tag_def Imply_def by (clarsimp simp add: \<phi>expns)
 
+lemma [\<phi>reason 1000 for \<open>?S \<^bold>i\<^bold>m\<^bold>p\<^bold>l\<^bold>i\<^bold>e\<^bold>s ?S' \<^bold>a\<^bold>n\<^bold>d ?V \<^bold><\<^bold>a\<^bold>c\<^bold>t\<^bold>i\<^bold>o\<^bold>n\<^bold>> collect_clean_value\<close>]:
+  \<open> X \<^bold>i\<^bold>m\<^bold>p\<^bold>l\<^bold>i\<^bold>e\<^bold>s X \<^bold>a\<^bold>n\<^bold>d True \<^bold><\<^bold>a\<^bold>c\<^bold>t\<^bold>i\<^bold>o\<^bold>n\<^bold>> collect_clean_value \<close>
+  unfolding Action_Tag_def using implies_refl .
 
 end
