Phi_Semantics/PhiSem_Variable_Lib.thy
@@ -1,19 +1,15 @@
 theory PhiSem_Variable_Lib
   imports PhiSem_Typed_Variable
+  keywords "val" :: quasi_command
 begin
 
 section \<open>Basic Operations\<close>
 
 subsection \<open>Variable\<close>
 
+(*
 
-proc
-  argument \<open>x \<Ztypecolon> \<^bold>v\<^bold>a\<^bold>l T\<heavy_comma> y \<Ztypecolon> \<^bold>v\<^bold>a\<^bold>l U\<close>
-  return \<open>xxxx\<close>
-  \<medium_left_bracket>
-  ;;  $\<a>\<r>\<g>1
-  ;; \<open>$1\<close> \<open>$(\<a>\<r>\<g>1)\<close>
-  ;; \<open>$2 := xx\<close>
+ *)
 
 subsubsection \<open>Syntax\<close>
 
@@ -42,11 +38,11 @@ parse_ast_translation \<open>
   end
 \<close> *)
 
-syntax "__get_var__" :: "idt \<Rightarrow> logic" ("$_" [1000] 999)
+(* syntax "__get_var__" :: "idt \<Rightarrow> logic" ("$_" [1000] 999)
 consts "get_var____\<phi>" :: "varname \<Rightarrow> 'b"
 
 translations "$x" => "CONST get_var____\<phi> x"
-
+*)
 
 lemma [\<phi>reason 2000 for
   \<open>Synthesis_Parse (?var::varname) (?Y::?'ret \<Rightarrow> assn)\<close>
@@ -84,18 +80,18 @@ consts infer_var_type :: \<open>unit action\<close>
 
 lemma [\<phi>reason 1000]:
   \<open> varname.type var \<equiv> TY'
-\<Longrightarrow> pred_option (\<lambda>TY'. TY = TY') TY' \<^bold><\<^bold>a\<^bold>c\<^bold>t\<^bold>i\<^bold>o\<^bold>n\<^bold>> infer_var_type
-\<Longrightarrow> pred_option (\<lambda>TY'. TY = TY') (varname.type var) \<^bold><\<^bold>a\<^bold>c\<^bold>t\<^bold>i\<^bold>o\<^bold>n\<^bold>> infer_var_type\<close>
+\<Longrightarrow> pred_option ((=) TY) TY' \<^bold><\<^bold>a\<^bold>c\<^bold>t\<^bold>i\<^bold>o\<^bold>n\<^bold>> infer_var_type
+\<Longrightarrow> pred_option ((=) TY) (varname.type var) \<^bold><\<^bold>a\<^bold>c\<^bold>t\<^bold>i\<^bold>o\<^bold>n\<^bold>> infer_var_type\<close>
   \<comment> \<open>TY is the output. The rule invokes evaluation of the \<open>varname.type var\<close>.\<close>
   by simp
 
 lemma [\<phi>reason 1000]:
-  \<open>pred_option (\<lambda>TY'. TY = TY') None \<^bold><\<^bold>a\<^bold>c\<^bold>t\<^bold>i\<^bold>o\<^bold>n\<^bold>> infer_var_type\<close>
+  \<open>pred_option ((=) TY) None \<^bold><\<^bold>a\<^bold>c\<^bold>t\<^bold>i\<^bold>o\<^bold>n\<^bold>> infer_var_type\<close>
   \<comment> \<open>the output TY can be anything freely\<close>
   by simp
 
-lemma [\<phi>reason 1000]:
-  \<open>pred_option (\<lambda>TY'. TY = TY') (Some TY) \<^bold><\<^bold>a\<^bold>c\<^bold>t\<^bold>i\<^bold>o\<^bold>n\<^bold>> infer_var_type\<close>
+lemma [\<phi>reason 1000 for \<open>pred_option ((=) ?TY') (Some ?TY) \<^bold><\<^bold>a\<^bold>c\<^bold>t\<^bold>i\<^bold>o\<^bold>n\<^bold>> infer_var_type\<close>]:
+  \<open>pred_option ((=) TY) (Some TY) \<^bold><\<^bold>a\<^bold>c\<^bold>t\<^bold>i\<^bold>o\<^bold>n\<^bold>> infer_var_type\<close>
   \<comment> \<open>the output TY equals to that TY in \<open>Some TY\<close> exactly.\<close>
   by simp
 
@@ -111,10 +107,13 @@ proc (nodef) op_set_var:
       \<open>\<phi>SemType (y \<Ztypecolon> U) TY\<close>
   argument \<open>x \<Ztypecolon> Var var T\<heavy_comma> \<^bold>v\<^bold>a\<^bold>l y \<Ztypecolon> U\<close>
   return   \<open>y \<Ztypecolon> \<^bold>v\<^bold>a\<^bold>r[var] U\<close>
-  \<medium_left_bracket> to_Identity \<open>var\<close> to_Identity op_set_var'' \<medium_right_bracket>. .
+  \<medium_left_bracket> to_Identity 
+    $y to_Identity
+    op_set_var'' 
+  \<medium_right_bracket>. .
 
 schematic_goal op_set_var__synthesis[
-  \<phi>reason for \<open>\<^bold>p\<^bold>r\<^bold>o\<^bold>c ?f \<lbrace> ?R \<longmapsto> \<lambda>ret. ?R'\<heavy_comma> SYNTHESIS ($?var := ?y) \<Ztypecolon> ?U ret \<^bold>t\<^bold>h\<^bold>r\<^bold>o\<^bold>w\<^bold>s ?E \<rbrace> \<^bold>@\<^bold>G\<^bold>O\<^bold>A\<^bold>L ?G\<close>
+  \<phi>reason for \<open>\<^bold>p\<^bold>r\<^bold>o\<^bold>c ?f \<lbrace> ?R \<longmapsto> \<lambda>ret. ?R'\<heavy_comma> SYNTHESIS (?y <set-to> ?var) \<Ztypecolon> ?U ret \<^bold>t\<^bold>h\<^bold>r\<^bold>o\<^bold>w\<^bold>s ?E \<rbrace> \<^bold>@\<^bold>G\<^bold>O\<^bold>A\<^bold>L ?G\<close>
 ]:
 assumes G: \<open>\<^bold>p\<^bold>r\<^bold>o\<^bold>c g \<lbrace> X \<longmapsto> X1\<heavy_comma> SYNTHESIS \<^bold>v\<^bold>a\<^bold>l y \<Ztypecolon> U \<^bold>t\<^bold>h\<^bold>r\<^bold>o\<^bold>w\<^bold>s E\<rbrace> \<^bold>@\<^bold>G\<^bold>O\<^bold>A\<^bold>L G \<close>
   and S[unfolded Action_Tag_def]:
@@ -122,15 +121,12 @@ assumes G: \<open>\<^bold>p\<^bold>r\<^bold>o\<^bold>c g \<lbrace> X \<longmapst
   and P: \<open>pred_option (\<lambda>TY'. TY = TY') (varname.type var) \<^bold><\<^bold>a\<^bold>c\<^bold>t\<^bold>i\<^bold>o\<^bold>n\<^bold>> infer_var_type\<close>
   and [\<phi>reason for \<open>\<phi>SemType (y \<Ztypecolon> U) ?TY\<close>]:
          \<open>\<phi>SemType (y \<Ztypecolon> U) TY\<close>
-shows \<open>\<^bold>p\<^bold>r\<^bold>o\<^bold>c ?FF \<lbrace> X \<longmapsto> Y\<heavy_comma> y \<Ztypecolon> \<^bold>v\<^bold>a\<^bold>r[var] U \<heavy_comma> SYNTHESIS \<^bold>v\<^bold>a\<^bold>l ($var := y) \<Ztypecolon> U \<^bold>t\<^bold>h\<^bold>r\<^bold>o\<^bold>w\<^bold>s E \<rbrace> \<^bold>@\<^bold>G\<^bold>O\<^bold>A\<^bold>L G\<close>
+shows \<open>\<^bold>p\<^bold>r\<^bold>o\<^bold>c ?FF \<lbrace> X \<longmapsto> Y\<heavy_comma> y \<Ztypecolon> \<^bold>v\<^bold>a\<^bold>r[var] U \<heavy_comma> SYNTHESIS \<^bold>v\<^bold>a\<^bold>l (y <set-to> var) \<Ztypecolon> U \<^bold>t\<^bold>h\<^bold>r\<^bold>o\<^bold>w\<^bold>s E \<rbrace> \<^bold>@\<^bold>G\<^bold>O\<^bold>A\<^bold>L G\<close>
   \<medium_left_bracket> G S op_set_var P op_get_var \<medium_right_bracket>. .
 
 
 
 paragraph \<open>Declare New Variables\<close>
-
-
-declare [[ML_print_depth=1000, eta_contract=false]]
 
 proc op_var_scope:
   assumes BLK: \<open>\<And>var. varname.type var \<equiv> TY
@@ -145,20 +141,68 @@ proc op_var_scope:
       BLK to_Identity op_free_var
     \<medium_right_bracket>.
     \<medium_left_bracket> to_Identity op_free_var throw \<medium_right_bracket>.
-  \<medium_right_bracket>. .
+    \<medium_right_bracket>. .
 
-lemma "__\<phi>op_set_var__":
+  thm op_var_scope_\<phi>compilation
+
+lemma "__set_var_rule__":
   \<open> \<^bold>p\<^bold>r\<^bold>o\<^bold>c g \<lbrace> R\<heavy_comma> y \<Ztypecolon> \<^bold>v\<^bold>a\<^bold>r[var] U\<heavy_comma> X \<longmapsto> Z \<^bold>t\<^bold>h\<^bold>r\<^bold>o\<^bold>w\<^bold>s E \<rbrace>
 \<Longrightarrow> pred_option (\<lambda>TY'. TY = TY') (varname.type var) \<^bold><\<^bold>a\<^bold>c\<^bold>t\<^bold>i\<^bold>o\<^bold>n\<^bold>> infer_var_type
 \<Longrightarrow> \<phi>SemType (y \<Ztypecolon> U) TY
-\<Longrightarrow> \<^bold>p\<^bold>r\<^bold>o\<^bold>c (op_set_var var TY raw \<ggreater> g) \<lbrace> R\<heavy_comma> (X\<heavy_comma> x \<Ztypecolon> Var var T \<heavy_comma> y \<Ztypecolon> Val raw U) \<longmapsto> Z \<^bold>t\<^bold>h\<^bold>r\<^bold>o\<^bold>w\<^bold>s E \<rbrace>\<close>
+\<Longrightarrow> \<^bold>p\<^bold>r\<^bold>o\<^bold>c (op_set_var var TY raw \<ggreater> g) \<lbrace> R\<heavy_comma> (X\<heavy_comma> x \<Ztypecolon> Var var T \<heavy_comma> y \<Ztypecolon> \<^bold>v\<^bold>a\<^bold>l[raw] U) \<longmapsto> Z \<^bold>t\<^bold>h\<^bold>r\<^bold>o\<^bold>w\<^bold>s E \<rbrace>\<close>
   \<medium_left_bracket> premises G and P and [\<phi>reason for \<open>\<phi>SemType (y \<Ztypecolon> U) ?TY\<close>]
     op_set_var P G \<medium_right_bracket>. .
 
-lemma "__\<phi>op_var_scope__0":
+lemma "__set_new_var_rule__":
+  \<open> (\<And>var. varname.type var \<equiv> Some TY
+              \<Longrightarrow> \<^bold>p\<^bold>r\<^bold>o\<^bold>c g \<lbrace> R\<heavy_comma> y \<Ztypecolon> \<^bold>v\<^bold>a\<^bold>r[var] U\<heavy_comma> X \<longmapsto> \<lambda>ret. Z ret \<heavy_comma> () \<Ztypecolon> Var var \<phi>Any
+                         \<^bold>t\<^bold>h\<^bold>r\<^bold>o\<^bold>w\<^bold>s \<lambda>e. E e\<heavy_comma> () \<Ztypecolon> Var var \<phi>Any \<rbrace>)
+\<Longrightarrow> \<phi>SemType (y \<Ztypecolon> U) TY
+\<Longrightarrow> \<^bold>p\<^bold>r\<^bold>o\<^bold>c op_var_scope TYPE('a) (Some TY) (\<lambda>var. op_set_var var TY raw \<ggreater> g)
+     \<lbrace> R\<heavy_comma> (X \<heavy_comma> y \<Ztypecolon> \<^bold>v\<^bold>a\<^bold>l[raw] U) \<longmapsto> Z \<^bold>t\<^bold>h\<^bold>r\<^bold>o\<^bold>w\<^bold>s E \<rbrace>\<close>
+  \<medium_left_bracket> premises G and [\<phi>reason]
+    op_var_scope[where TY=\<open>Some TY\<close>] \<medium_left_bracket> premises [\<phi>reason for \<open>varname.type var \<equiv> _\<close>]
+      $y op_set_var G
+    \<medium_right_bracket>.
+  \<medium_right_bracket>. .
+
+lemma "__set_new_var_noty_rule__":
+  \<open> (\<And>var. varname.type var \<equiv> None
+              \<Longrightarrow> \<^bold>p\<^bold>r\<^bold>o\<^bold>c g \<lbrace> R\<heavy_comma> y \<Ztypecolon> \<^bold>v\<^bold>a\<^bold>r[var] U\<heavy_comma> X \<longmapsto> \<lambda>ret. Z ret \<heavy_comma> () \<Ztypecolon> Var var \<phi>Any
+                         \<^bold>t\<^bold>h\<^bold>r\<^bold>o\<^bold>w\<^bold>s \<lambda>e. E e\<heavy_comma> () \<Ztypecolon> Var var \<phi>Any \<rbrace>)
+\<Longrightarrow> \<phi>SemType (y \<Ztypecolon> U) TY
+\<Longrightarrow> \<^bold>p\<^bold>r\<^bold>o\<^bold>c op_var_scope TYPE('a) None (\<lambda>var. op_set_var var TY raw \<ggreater> g)
+     \<lbrace> R\<heavy_comma> (X \<heavy_comma> y \<Ztypecolon> \<^bold>v\<^bold>a\<^bold>l[raw] U) \<longmapsto> Z \<^bold>t\<^bold>h\<^bold>r\<^bold>o\<^bold>w\<^bold>s E \<rbrace>\<close>
+  \<medium_left_bracket> premises G and [\<phi>reason for \<open>\<phi>SemType (y \<Ztypecolon> U) _\<close>]
+    op_var_scope[where TY=None] \<medium_left_bracket> premises [\<phi>reason for \<open>varname.type var \<equiv> _\<close>]
+      $y op_set_var G
+    \<medium_right_bracket>.
+  \<medium_right_bracket>. .
+
+
+lemma "__value_access_0__":
   \<open> \<^bold>p\<^bold>r\<^bold>o\<^bold>c F \<lbrace> R \<longmapsto> Y \<^bold>t\<^bold>h\<^bold>r\<^bold>o\<^bold>w\<^bold>s E \<rbrace>
 \<Longrightarrow> \<^bold>p\<^bold>r\<^bold>o\<^bold>c F \<lbrace> R\<heavy_comma> Void \<longmapsto> Y \<^bold>t\<^bold>h\<^bold>r\<^bold>o\<^bold>w\<^bold>s E \<rbrace>\<close>
   by fastforce
+
+lemma
+  \<open> \<^bold>p\<^bold>r\<^bold>o\<^bold>c Return \<phi>V_none \<lbrace> X \<longmapsto> \<lambda>_. Y \<^bold>t\<^bold>h\<^bold>r\<^bold>o\<^bold>w\<^bold>s Any \<rbrace>
+\<Longrightarrow> \<^bold>v\<^bold>i\<^bold>e\<^bold>w X \<longmapsto> Y\<close>
+  unfolding \<phi>Procedure_def View_Shift_def Return_def det_lift_def
+  by (simp add: \<phi>expns)
+
+lemma
+  \<open> (sem_value.dest v \<in> (x \<Ztypecolon> T) \<Longrightarrow> \<^bold>p\<^bold>r\<^bold>o\<^bold>c F \<lbrace> R \<longmapsto> R' \<^bold>t\<^bold>h\<^bold>r\<^bold>o\<^bold>w\<^bold>s E \<rbrace>)
+\<Longrightarrow> \<^bold>p\<^bold>r\<^bold>o\<^bold>c F \<lbrace> R\<heavy_comma> x \<Ztypecolon> \<^bold>v\<^bold>a\<^bold>l[v] T \<longmapsto> R' \<^bold>t\<^bold>h\<^bold>r\<^bold>o\<^bold>w\<^bold>s E \<rbrace>\<close>
+  unfolding \<phi>Procedure_def
+  by (clarsimp simp add: \<phi>expns)
+
+
+lemma
+  \<open> \<^bold>p\<^bold>r\<^bold>o\<^bold>c F \<lbrace> R \<longmapsto> R' \<^bold>t\<^bold>h\<^bold>r\<^bold>o\<^bold>w\<^bold>s E \<rbrace>
+\<Longrightarrow> \<^bold>p\<^bold>r\<^bold>o\<^bold>c F \<lbrace> R\<heavy_comma> x \<Ztypecolon> \<^bold>v\<^bold>a\<^bold>l[v] T \<longmapsto> \<lambda>ret. R' ret \<^bold>s\<^bold>u\<^bold>b\<^bold>j sem_value.dest v \<in> (x \<Ztypecolon> T) \<^bold>t\<^bold>h\<^bold>r\<^bold>o\<^bold>w\<^bold>s E \<rbrace>\<close>
+  unfolding \<phi>Procedure_def
+  by (clarsimp simp add: \<phi>expns)
 
 
 thm "__\<phi>op_set_var__"[OF "__\<phi>op_set_var__" [OF "__\<phi>op_var_scope__0"]]
@@ -174,5 +218,19 @@ ML_file_debug "library/local_value.ML"
   raise NuProcessor.Terminate_Process (Local_Value.mk_var_scope vars (ctxt,sequent), I)))
 \<close>
 
+lemma [\<phi>reason 1]:
+  \<open>FAIL TEXT(\<open>Fail to reason the semantic type of\<close> X)
+\<Longrightarrow> \<phi>SemType X Any\<close>
+  by blast
+
+proc
+  assumes [\<phi>reason for \<open>\<phi>SemType (x \<Ztypecolon> T) _ \<close>]: \<open>\<phi>SemType (x \<Ztypecolon> T) TY\<close>
+  argument \<open>x \<Ztypecolon> \<^bold>v\<^bold>a\<^bold>l T\<heavy_comma> y \<Ztypecolon> \<^bold>v\<^bold>a\<^bold>l U\<close>
+  return \<open>xxxx\<close>
+  \<medium_left_bracket>
+  ;; $x \<rightarrow> xx
+  ;;  $\<a>\<r>\<g>1
+  ;; \<open>$1\<close> \<open>$(\<a>\<r>\<g>1)\<close>
+  ;; \<open>$2 := xx\<close>
 
 end
